\documentclass[12pt,letterpaper]{article}
\usepackage[utf8]{inputenc}
\usepackage[english]{babel}
\usepackage{amsmath}
\usepackage[letterpaper,margin=0.6in]{geometry}
\usepackage{fancyhdr}
\usepackage{float}
\usepackage{tkz-euclide}


\newcommand\lreqn[2]{\noindent\makebox[\textwidth]{$\displaystyle#1$\hfill(#2)}\vspace{2ex}}

\pagestyle{empty}
\pagestyle{fancy}
\fancyhf{}
\lhead{Name:}
\rhead{\textit{December 8, 2020}}

\begin{document}

\section*{Pythagorean Triples}

Pythagorean triples are sets of positive whole numbers whichb satisfy the pythagorean theorem.
We can generate them using the following method.

\noindent First, choose whole numbers $n$ and $m$ such that $m > n$, then:

\begin{align*} 
a &= m^2 - n^2 \\
b &= 2nm \\
c &= m^2 + n^2 
\end{align*}

\subsection*{Generating some triples}

Following the formulae above for calculating $a$, $b$, and $c$, generate these triples.

\begin{table}[ht]
  \begin{tabular}{c|c|c|c|c}
     $n$ & $m$ & $a = m^2 - n^2$ & $b = 2nm$ & $c = m^2 + n^2$ \\
      \hline
      1  &  2  &   &   &   \\
      1  &  3  &   &   &   \\
      2  &  3  &   &   &   \\
  \end{tabular}
\end{table}

\subsection*{Prove using Algebra}

Put $a^2 + b^2$ with the foumlae above in simplest form:

\begin{align*}
 a^2 + b^2 &= (m^2 -n^2)^2 + (2nm)^2 \\
           &= (m^2 - n^2)(m^2 - n^2) + (2nm)(2nm) \\
           &= m^2(m^2 - n^2) - n^2(m^2 - n^2) + 4n^2m^2 \\
           &= m^4 - n^2m^2  -n^2m^2 + n^4 + 4n^2m^2 \\
           &= m^4 + n^4 + 2n^2m^2
\end{align*}

\noindent Put $c^2$ in simplest form:

\begin{align*}
 c^2 &= (m^2 + n^2)^2 \\
     &= (m^2 + n^2)(m^2 + n^2) \\
     &= m^2(m^2 + n^2) + n^2(m^2 + n^2) \\
     &= m^4 + n^2m^2 + n^2m^2 + n^4 \\
     &= m^4 + n^4 + 2n^2m^2
\end{align*}

\end{document}